commit

AP/AP/Basic.lean
@@ -56,12 +56,18 @@ theorem dState_def {s : State} : s.DState ↔ s.WF ∧ s.aTurn = false :=
   ⟨λ ⟨h₁, h₂⟩ => ⟨h₁, h₂⟩, λ ⟨h₁, h₂⟩ => ⟨h₁, h₂⟩⟩
 
 def State.dChooseMove (s : State) : PointZ :=
-  (insert s.a_pos s.taken).max! + ⟨1, 0⟩
+  (insert s.aPos s.taken).max! + ⟨1, 0⟩
 
 @[simp]
-theorem a_wf_tr_iff {s : State} [hs : s.AState] {p} :
-sys.validTr s p ↔ s.a_pos ≠ p ∧ p ∉ s.taken ∧ p.dist s.a_pos ≤ s.pw := by
-  rcases hs with ⟨hs, ht⟩
+theorem State.AState.turn {s : State} [hs : s.AState] : s.aTurn := by
+  cases hs; assumption
+
+@[simp]
+theorem State.DState.turn {s : State} [hs : s.DState] : s.aTurn = false := by
+  cases hs; assumption
+
+theorem State.validTr_iff_of_aTurn {s : State} {p} (ht : s.aTurn) :
+sys.validTr s p ↔ s.aPos ≠ p ∧ p ∉ s.taken ∧ p.dist s.aPos ≤ s.pw := by
   constructor
   · rintro ⟨s', h₁⟩
     simp [sys, State.move, State.aMove, ht] at h₁
@@ -71,10 +77,8 @@ sys.validTr s p ↔ s.a_pos ≠ p ∧ p ∉ s.taken ∧ p.dist s.a_pos ≤ s.pw 
     use (s.move p).get!
     simp [sys, State.move, State.aMove, ht, h]
 
-@[simp]
-theorem d_wf_tr_iff {s : State} [hs : s.DState] {p} :
-sys.validTr s p ↔ s.a_pos ≠ p ∧ p ∉ s.taken := by
-  rcases hs with ⟨hs, ht⟩
+theorem State.validTr_iff_of_not_aTurn {s : State} {p} (ht : s.aTurn = false) :
+sys.validTr s p ↔ s.aPos ≠ p ∧ p ∉ s.taken := by
   constructor
   · rintro ⟨s', h₁⟩
     simp [sys, State.move, State.dMove, ht] at h₁
@@ -85,12 +89,156 @@ sys.validTr s p ↔ s.a_pos ≠ p ∧ p ∉ s.taken := by
     simp [sys, State.move, State.dMove, ht, h]
 
 @[simp]
-theorem State.DState.hasTr {s : State} [hs : s.DState] : sys.hasTr s := by
-  use s.dChooseMove; simp
-  suffices h₁ : s.dChooseMove ∉  insert s.a_pos s.taken
-  · simp at h₁; rw [eq_comm]; exact h₁
+theorem State.AState.validTr_iff {s : State} [hs : s.AState] {p} :
+sys.validTr s p ↔ s.aPos ≠ p ∧ p ∉ s.taken ∧ p.dist s.aPos ≤ s.pw := by
+  apply s.validTr_iff_of_aTurn; simp
+
+@[simp]
+theorem State.DState.validTr_iff {s : State} [hs : s.DState] {p} :
+sys.validTr s p ↔ s.aPos ≠ p ∧ p ∉ s.taken := by
+  apply s.validTr_iff_of_not_aTurn; simp
+
+theorem State.validTr_dChooseMove {s : State} (ht : s.aTurn = false) :
+sys.validTr s s.dChooseMove := by
+  rw [s.validTr_iff_of_not_aTurn ht]
+  suffices h₁ : s.dChooseMove ∉ insert s.aPos s.taken
+  · simp at h₁; rw [ne_comm]; exact h₁
   apply Set'.not_mem_of_max!_lt
   simp [State.dChooseMove, Point.zero_def]
 
-theorem d_has_move {s : State} [hs : s.DState] : sys.hasTr s :=
-  hs.hasTr
+theorem State.hasTr_of_not_aTurn {s : State} (ht : s.aTurn = false) : sys.hasTr s := by
+  use s.dChooseMove; exact s.validTr_dChooseMove ht
+
+@[simp]
+theorem State.DState.hasTr {s : State} [hs : s.DState] : sys.hasTr s := by
+  apply s.hasTr_of_not_aTurn; simp
+
+def State.aMoves (s : State) : List PointZ := do
+  let ⟨ax, ay⟩ := s.aPos
+  let ds := List.map (Int.ofNat · - s.pw) #
+    List.range # s.pw * 2 + 1
+  let x ← ds
+  let y ← ds
+  let p := ⟨ax + x, ay + y⟩
+  guard # sys.validTr s p
+  return p
+
+def State.aHasMove (s : State) : Bool :=
+  s.aMoves ≠ []
+
+theorem State.hasTr_iff_of_aTurn {s : State} (ht : s.aTurn) :
+sys.hasTr s ↔ ∃ p, s.aPos ≠ p ∧ p ∉ s.taken ∧ p.dist s.aPos ≤ s.pw := by
+  simp [sys, System.hasTr_iff, move, aMove, ht]
+
+@[simp]
+theorem State.AState.hasTr_iff {s : State} [hs : s.AState] :
+sys.hasTr s ↔ ∃ p, s.aPos ≠ p ∧ p ∉ s.taken ∧ p.dist s.aPos ≤ s.pw := by
+  simp [s.hasTr_iff_of_aTurn]
+
+theorem State.aHasMove_of_hasTr {s : State}
+(ht : s.aTurn) (h : sys.hasTr s) : s.aHasMove := by
+  simp [aHasMove, aMoves, s.hasTr_iff_of_aTurn ht] at h ⊢
+  simp [sys, move, aMove, ht]; clear ht
+  rcases h with ⟨p, h₁, h₂, h₃⟩
+  use Int.toNat # s.pw + p.x - s.aPos.x
+  constructor
+  rotate_left
+  use Int.toNat # s.pw + p.y - s.aPos.y
+  constructor
+  any_goals
+    clear h₁ h₂
+    cases s; nm pw taken aPos aTurn hist
+    simp [PointZ.dist] at h₃ ⊢
+    rw [←Int.le_iff_lt_add_one]
+    rcases h₃ with ⟨h₁, h₂⟩
+    rw [Int.add_sub_assoc, mul_two]
+    simp
+    replace h₁ := le_of_max_le_left h₁
+    replace h₂ := le_of_max_le_left h₂
+    linarith
+  simp
+  cases s; nm pw taken aPos aTurn hist
+  constructor
+  · simp [PointZ.dist] at h₁ h₃ ⊢; clear h₂
+    convert h₁ <;> rcases h₃ with ⟨h₁, h₂⟩
+    · have h₃ : max (pw + p.x - aPos.x) 0 = pw + p.x - aPos.x := by
+        apply max_eq_left
+        replace h₁ := le_of_max_le_right h₁
+        linarith
+      rw [h₃]
+      ring
+    · have h₃ : max (pw + p.y - aPos.y) 0 = pw + p.y - aPos.y := by
+        apply max_eq_left
+        replace h₂ := le_of_max_le_right h₂
+        linarith
+      rw [h₃]
+      ring
+  constructor
+  · simp [PointZ.dist] at h₃ ⊢
+    dsimp at h₁ h₂
+    rcases h₃ with ⟨h₅, h₆⟩
+    replace h₅ : max (pw + p.x - aPos.x) 0 = pw + p.x - aPos.x := by
+      apply max_eq_left
+      replace h₅ := le_of_max_le_right h₅
+      linarith
+    replace h₆ : max (pw + p.y - aPos.y) 0 = pw + p.y - aPos.y := by
+      apply max_eq_left
+      replace h₆ := le_of_max_le_right h₆
+      linarith
+    simp [h₅, h₆]
+    ring_nf
+    exact h₂
+  dsimp at h₁ h₂ h₃ ⊢
+  rw [PointZ.dist.comm]
+  convert h₃
+  · simp [PointZ.dist] at h₃
+    rcases h₃ with ⟨h₃, h₄⟩
+    replace h₃ : max (pw + p.x - aPos.x) 0 = pw + p.x - aPos.x := by
+      apply max_eq_left
+      replace h₃ := le_of_max_le_right h₃
+      linarith
+    rw [h₃]
+    linarith
+  · simp [PointZ.dist] at h₃
+    rcases h₃ with ⟨h₃, h₄⟩
+    replace h₄ : max (pw + p.y - aPos.y) 0 = pw + p.y - aPos.y := by
+      apply max_eq_left
+      replace h₄ := le_of_max_le_right h₄
+      linarith
+    rw [h₄]
+    linarith
+
+theorem State.hasTr_of_aHasMove {s : State} (ht : s.aTurn)
+(h : s.aHasMove) : sys.hasTr s := by
+  simp [aHasMove, aMoves, s.hasTr_iff_of_aTurn ht] at h ⊢
+  simp [sys, move, aMove, ht] at h
+  rcases h with ⟨x, hx, y, hy, h₁⟩
+  rcases h₁ with ⟨h₁, h₂, h₃⟩
+  use ⟨s.aPos.x + (x - s.pw), s.aPos.y + (y - s.pw)⟩
+  use h₁, h₂
+  rw [PointZ.dist.comm]
+  exact h₃
+
+theorem State.hasTr_iff_aHasMove {s : State} (ht : s.aTurn) :
+sys.hasTr s ↔ s.aHasMove := ⟨s.aHasMove_of_hasTr ht, s.hasTr_of_aHasMove ht⟩
+
+theorem State.WF.ind_turn {P : State → Prop}
+(h₁ : ∀ (s : State), s.AState → P s) (h₂ : ∀ (s : State), s.DState → P s)
+{s : State} (hs : s.WF) : P s := by
+  cases ht : s.aTurn
+  · apply h₂; constructor <;> assumption
+  · apply h₁; constructor <;> assumption
+
+@[simp]
+def State.hasMove (s : State) : Bool :=
+  if s.aTurn then s.aHasMove else true
+
+theorem State.hasTr_iff_hasMove {s : State} : sys.hasTr s ↔ s.hasMove := by
+  simp; cases ht : s.aTurn <;> simp
+  · exact hasTr_of_not_aTurn ht
+  · exact hasTr_iff_aHasMove ht
+
+instance {s : State} : Decidable (sys.hasTr s) :=
+  match h : s.hasMove with
+  | true => .isTrue # by rwa [s.hasTr_iff_hasMove]
+  | false => .isFalse # by rw [s.hasTr_iff_hasMove, h]; simp
