AP/System/Invariant.lean
@@ -7,7 +7,7 @@ variable {S T : Type u} {sys : System S T}
 
 theorem invariant {p : S → Prop} {a b}
 (h₁ : p a) (h₂ : sys.Reachable a b)
-(h₃ : ∀ {x y t}, p x → sys.trTo x t y → p y) : p b := by
+(h₃ : ∀ {x y t}, p x → sys.tr x t = some y → p y) : p b := by
   induction h₂; exact h₁
   clear a b
   nm a b c t h₂ h₄ ih
@@ -16,13 +16,13 @@ theorem invariant {p : S → Prop} {a b}
 
 theorem invariant_init {p : S → Prop} {a}
 (h₁ : sys.WF a) (h₂ : ∀ {a}, sys.Initial a → p a)
-(h₃ : ∀ {x y t}, p x → sys.trTo x t y → p y) : p a := by
+(h₃ : ∀ {x y t}, p x → sys.tr x t = some y → p y) : p a := by
   rw [wf_iff] at h₁
   obtain ⟨s₀, h₁, h₄⟩ := h₁
   exact invariant (h₂ h₁) h₄ h₃
 
 theorem invariant_val {α : Type*} {a b} {f : S → α} (h₁ : sys.Reachable a b)
-(h₂ : ∀ {x y t}, sys.trTo x t y → f y = f x) : f b = f a := by
+(h₂ : ∀ {x y t}, sys.tr x t = some y → f y = f x) : f b = f a := by
   apply invariant (p := (f · = f a)) rfl h₁
   intro x y t h₃ h₄
   rw [←h₃]
