AP/Util/Logic.lean
@@ -146,8 +146,10 @@ theorem inst_decidableEq_eq {α : Type*} {H₁ H₂ : DecidableEq α} : H₁ = H
   inst_decidableRel_eq
 
 theorem forall_iff_of {α : Sort*} {p q : α → Prop}
-(h : ∀ x, p x ↔ q x) : (∀ x, p x) ↔ (∀ x, q x) := by
-  simp [h]
+(h : ∀ x, p x ↔ q x) : (∀ x, p x) ↔ (∀ x, q x) := by simp [h]
+
+theorem exists_iff_of {α : Sort*} {p q : α → Prop}
+(h : ∀ x, p x ↔ q x) : (∃ x, p x) ↔ (∃ x, q x) := by simp [h]
 
 theorem iff_of_isEquiv {α : Type*} {r : α → α → Prop}
 [hr : IsEquiv α r] {a b c d : α} (h₁ : r a c) (h₂ : r b d) :
